update coq proofs for name changes in Map and Array
(sorry for not doing it earlier)

examples/programs/decrease1/decrease1.mlw_Decrease1_decrease1_induction_2.v
@@ -4,13 +4,9 @@ Require Import ZArith.
 Require Import Rbase.
 Definition unit  := unit.
 
-Parameter ignore: forall (a:Type), a  -> unit.
+Parameter label : Type.
 
-Implicit Arguments ignore.
-
-Parameter label_ : Type.
-
-Parameter at1: forall (a:Type), a -> label_  -> a.
+Parameter at1: forall (a:Type), a -> label  -> a.
 
 Implicit Arguments at1.
 
@@ -30,22 +26,21 @@ Implicit Arguments contents.
 
 Parameter map : forall (a:Type) (b:Type), Type.
 
-Parameter mixfix_lbrb: forall (a:Type) (b:Type), (map a b) -> a  -> b.
+Parameter get: forall (a:Type) (b:Type), (map a b) -> a  -> b.
 
-Implicit Arguments mixfix_lbrb.
+Implicit Arguments get.
 
-Parameter mixfix_lblsmnrb: forall (a:Type) (b:Type), (map a b) -> a -> b  ->
-  (map a b).
+Parameter set: forall (a:Type) (b:Type), (map a b) -> a -> b  -> (map a b).
 
-Implicit Arguments mixfix_lblsmnrb.
+Implicit Arguments set.
 
 Axiom Select_eq : forall (a:Type) (b:Type), forall (m:(map a b)),
-  forall (a1:a) (a2:a), forall (b1:b), (a1 = a2) ->
-  ((mixfix_lbrb (mixfix_lblsmnrb m a1 b1) a2) = b1).
+  forall (a1:a) (a2:a), forall (b1:b), (a1 = a2) -> ((get (set m a1 b1)
+  a2) = b1).
 
 Axiom Select_neq : forall (a:Type) (b:Type), forall (m:(map a b)),
-  forall (a1:a) (a2:a), forall (b1:b), (~ (a1 = a2)) ->
-  ((mixfix_lbrb (mixfix_lblsmnrb m a1 b1) a2) = (mixfix_lbrb m a2)).
+  forall (a1:a) (a2:a), forall (b1:b), (~ (a1 = a2)) -> ((get (set m a1 b1)
+  a2) = (get m a2)).
 
 Parameter const: forall (b:Type) (a:Type), b  -> (map a b).
 
@@ -53,8 +48,8 @@ Set Contextual Implicit.
 Implicit Arguments const.
 Unset Contextual Implicit.
 
-Axiom Const : forall (b:Type) (a:Type), forall (b1:b) (a1:a),
-  ((mixfix_lbrb (const(b1):(map a b)) a1) = b1).
+Axiom Const : forall (b:Type) (a:Type), forall (b1:b) (a1:a), ((get (const(
+  b1):(map a b)) a1) = b1).
 
 Inductive array (a:Type) :=
   | mk_array : Z -> (map Z a) -> array a.
@@ -72,24 +67,22 @@ Definition length (a:Type)(u:(array a)): Z :=
   end.
 Implicit Arguments length.
 
-Definition mixfix_lbrb1 (a:Type)(a1:(array a)) (i:Z): a :=
-  (mixfix_lbrb (elts a1) i).
-Implicit Arguments mixfix_lbrb1.
+Definition get1 (a:Type)(a1:(array a)) (i:Z): a := (get (elts a1) i).
+Implicit Arguments get1.
 
-Definition mixfix_lblsmnrb1 (a:Type)(a1:(array a)) (i:Z) (v:a): (array a) :=
+Definition set1 (a:Type)(a1:(array a)) (i:Z) (v:a): (array a) :=
   match a1 with
-  | mk_array xcl0 _ => (mk_array xcl0 (mixfix_lblsmnrb (elts a1) i v))
+  | mk_array xcl0 _ => (mk_array xcl0 (set (elts a1) i v))
   end.
-Implicit Arguments mixfix_lblsmnrb1.
+Implicit Arguments set1.
 
 Definition decrease1(a:(array Z)): Prop := forall (i:Z), ((0%Z <= i)%Z /\
-  (i <  ((length a) - 1%Z)%Z)%Z) -> (((mixfix_lbrb1 a
-  i) - 1%Z)%Z <= (mixfix_lbrb1 a (i + 1%Z)%Z))%Z.
+  (i <  ((length a) - 1%Z)%Z)%Z) -> (((get1 a i) - 1%Z)%Z <= (get1 a
+  (i + 1%Z)%Z))%Z.
 
 Theorem decrease1_induction : forall (a:(array Z)), (decrease1 a) ->
   forall (i:Z) (j:Z), (((0%Z <= i)%Z /\ (i <= j)%Z) /\
-  (j <  (length a))%Z) -> ((((mixfix_lbrb1 a
-  i) + i)%Z - j)%Z <= (mixfix_lbrb1 a j))%Z.
+  (j <  (length a))%Z) -> ((((get1 a i) + i)%Z - j)%Z <= (get1 a j))%Z.
 (* YOU MAY EDIT THE PROOF BELOW *)
 unfold decrease1.
 intros a Ha i j Hij.
@@ -102,11 +95,11 @@ destruct H4.
 subst x.
 ring_simplify.
 omega.
-apply Zle_trans with (mixfix_lbrb1 a (x-1) - 1)%Z.
+apply Zle_trans with (get1 a (x-1) - 1)%Z.
 assert (i <= x-1 < x)%Z by omega.
 assert (0 <= i <= x-1 /\ x-1 < length a)%Z by omega.
 generalize (H (x-1)%Z H8 H9); clear H; intuition.
-apply Zle_trans with (mixfix_lbrb1 a (x-1+1))%Z.
+apply Zle_trans with (get1 a (x-1+1))%Z.
 apply (Ha (x-1)%Z); omega.
 ring_simplify (x-1+1)%Z.
 omega.
